Foundation/Modal/Kripke/Logic/Triv.lean
@@ -1,6 +1,4 @@
-import Foundation.Modal.Kripke.Logic.KT
 import Foundation.Modal.Kripke.Logic.KTc
-import Foundation.Modal.Kripke.Rooted
 import Foundation.Modal.Kripke.Logic.GrzPoint3
 import Foundation.Modal.Kripke.Logic.S4Point4M
 import Foundation.Vorspiel.HRel.Equality
@@ -13,86 +11,73 @@ open Hilbert.Kripke
 
 namespace Kripke
 
-protected abbrev FrameClass.refl_corefl : FrameClass := { F | F.IsReflexive ∧ IsCoreflexive _ F }
-protected abbrev FrameClass.equality : FrameClass := { F | IsEquality _ F }
-protected abbrev FrameClass.finite_equality : FrameClass := { F | Finite F.World ∧ IsEquality _ F }
+variable {F : Frame}
 
-lemma FrameClass.eq_equality_refl_corefl : Kripke.FrameClass.equality = Kripke.FrameClass.refl_corefl := by
-  ext F;
-  constructor;
-  . intro F_eq;
-    replace F_eq := Set.mem_setOf_eq.mp F_eq;
+protected abbrev Frame.IsTriv (F : Frame) := _root_.IsEquality F.Rel
+instance [F.IsTriv] : F.IsS4Point4M where
+  mckinsey := by simp
 
-  . rintro ⟨hRefl, hCorefl⟩;
-    apply Set.mem_setOf_eq.mpr;
-    infer_instance;
+protected class Frame.IsFiniteTriv (F : Frame) extends F.IsFinite, F.IsTriv
+instance [F.IsFiniteTriv] : F.IsFiniteGrzPoint3 where
+
+@[simp] lemma Frame.equality [F.IsTriv] {x y : F} : x ≺ y ↔ x = y := by apply _root_.equality;
+
+protected abbrev FrameClass.Triv : FrameClass := { F | F.IsTriv }
+protected abbrev FrameClass.finite_Triv : FrameClass := { F | F.IsFiniteTriv }
+
 
 end Kripke
 
 
 namespace Hilbert.Triv.Kripke
 
-instance sound_refl_corefl : Sound (Hilbert.Triv) Kripke.FrameClass.refl_corefl :=
+instance sound_Triv : Sound (Hilbert.Triv) Kripke.FrameClass.Triv :=
+  instSound_of_validates_axioms $ by
+    apply FrameClass.Validates.withAxiomK;
+    rintro F ⟨_⟩ _ (rfl | rfl);
+    . exact validate_AxiomT_of_reflexive;
+    . exact validate_AxiomTc_of_coreflexive;
+
+instance sound_finite_Triv : Sound (Hilbert.Triv) Kripke.FrameClass.finite_Triv :=
   instSound_of_validates_axioms $ by
     apply FrameClass.Validates.withAxiomK;
     rintro F ⟨_, _⟩ _ (rfl | rfl);
     . exact validate_AxiomT_of_reflexive;
     . exact validate_AxiomTc_of_coreflexive;
 
-instance sound_equality : Sound (Hilbert.Triv) Kripke.FrameClass.equality := by
-  convert sound_refl_corefl;
-  rw [Kripke.FrameClass.eq_equality_refl_corefl];
-
-instance sound_finite_equality : Sound (Hilbert.Triv) Kripke.FrameClass.finite_equality :=
-  instSound_of_validates_axioms $ by
-    apply FrameClass.Validates.withAxiomK;
-    rintro F ⟨_, _⟩ _ (rfl | rfl);
-    . exact validate_AxiomT_of_reflexive;
-    . exact validate_AxiomTc_of_coreflexive;
-
-instance consistent : Entailment.Consistent (Hilbert.Triv) := consistent_of_sound_frameclass Kripke.FrameClass.refl_corefl $ by
+instance consistent : Entailment.Consistent (Hilbert.Triv) := consistent_of_sound_frameclass Kripke.FrameClass.Triv $ by
   use whitepoint;
+  constructor;
 
+instance cannonical_Triv : Canonical (Hilbert.Triv) Kripke.FrameClass.Triv := ⟨by constructor⟩
 
-
-instance cannonical_refl_corefl : Canonical (Hilbert.Triv) Kripke.FrameClass.refl_corefl := ⟨by
-  apply Set.mem_setOf_eq.mpr;
-
-⟩
-
-instance complete_refl_corefl : Complete (Hilbert.Triv) Kripke.FrameClass.refl_corefl := inferInstance
-
-instance complete_equality : Complete (Hilbert.Triv) Kripke.FrameClass.equality := by
-  rw [Kripke.FrameClass.eq_equality_refl_corefl];
-  infer_instance;
-
+instance complete_Triv : Complete (Hilbert.Triv) Kripke.FrameClass.Triv := inferInstance
 
 section FFP
 
 open Relation in
-instance complete_finite_equality : Complete (Hilbert.Triv) Kripke.FrameClass.finite_equality := ⟨by
+instance complete_finite_Triv : Complete (Hilbert.Triv) Kripke.FrameClass.finite_Triv := ⟨by
   intro φ hφ;
-  apply Kripke.complete_equality.complete;
+  apply Kripke.complete_Triv.complete;
   intro F F_eq V r;
   replace F_eq := Set.mem_setOf_eq.mp F_eq;
   apply Model.pointGenerate.modal_equivalent_at_root (r := r) |>.mp;
   apply hφ;
-  refine ⟨?_, ?_⟩;
-  . apply finite_iff_exists_equiv_fin.mpr;
-    use 1;
-    constructor;
-    trans Unit;
-    . refine ⟨λ _ => (), λ _ => ⟨r, by tauto⟩, ?_, ?_⟩
-      . simp only [Function.LeftInverse, Subtype.forall, Subtype.mk.injEq, forall_eq_or_imp, true_and];
-        intro x Rrx;
-        exact IsEquality.equality.mp $ Relation.TransGen.unwrap Rrx
-      . simp [Function.RightInverse, Function.LeftInverse];
-    . exact finOneEquiv.symm;
-  . apply isEquality_iff _ _ |>.mpr;
-    rintro ⟨x, (rfl | hx)⟩ ⟨y, (rfl | hy)⟩;
-    . simp [IsRefl.refl];
-    all_goals
-    . simp only [Subtype.mk.injEq]; apply IsEquality.equality;
+  exact {
+    world_finite := by
+      apply finite_iff_exists_equiv_fin.mpr;
+      use 1;
+      constructor;
+      trans Unit;
+      . refine ⟨λ _ => (), λ _ => ⟨r, by tauto⟩, ?_, ?_⟩
+        . simp only [Function.LeftInverse, Subtype.forall, Subtype.mk.injEq, forall_eq_or_imp, true_and];
+          intro x Rrx;
+          exact Frame.equality.mp $ Rrx.unwrap
+        . simp [Function.RightInverse, Function.LeftInverse];
+      . exact finOneEquiv.symm;
+    refl := by simp;
+    corefl := by rintro ⟨x⟩ ⟨y⟩ Rxy; simpa [Subtype.mk.injEq] using Rxy;
+  }
 ⟩
 
 end FFP
@@ -107,8 +92,8 @@ open Entailment
 open Kripke
 
 
-lemma Triv.Kripke.equality : Logic.Triv = FrameClass.equality.logic := eq_hilbert_logic_frameClass_logic
-lemma Triv.Kripke.finite_equality : Logic.Triv = FrameClass.finite_equality.logic := eq_hilbert_logic_frameClass_logic
+lemma Triv.Kripke.equality : Logic.Triv = FrameClass.Triv.logic := eq_hilbert_logic_frameClass_logic
+lemma Triv.Kripke.finite_equality : Logic.Triv = FrameClass.finite_Triv.logic := eq_hilbert_logic_frameClass_logic
 
 @[simp]
 theorem Triv.proper_extension_of_KTc : Logic.KTc ⊂ Logic.Triv := by
@@ -130,9 +115,10 @@ theorem Triv.proper_extension_of_KTc : Logic.KTc ⊂ Logic.Triv := by
 theorem Triv.proper_extension_of_GrzPoint3 : Logic.GrzPoint3 ⊂ Logic.Triv := by
   constructor;
   . rw [GrzPoint3.Kripke.finite_connected_partial_order, Triv.Kripke.finite_equality];
-    rintro φ hφ F ⟨_, _⟩;
+    rintro φ hφ F hF;
     apply hφ;
-    refine ⟨by tauto, inferInstance, inferInstance⟩;
+    simp_all only [Set.mem_setOf_eq];
+    infer_instance;
   . suffices ∃ φ, Hilbert.Triv ⊢! φ ∧ ¬FrameClass.finite_connected_partial_order ⊧ φ by
       rw [GrzPoint3.Kripke.finite_connected_partial_order];
       tauto;
@@ -143,25 +129,24 @@ theorem Triv.proper_extension_of_GrzPoint3 : Logic.GrzPoint3 ⊂ Logic.Triv := b
       let M : Model := ⟨⟨Fin 2, λ x y => x ≤ y⟩, (λ w _ => w = 0)⟩;
       use M, 0;
       constructor;
-      . refine ⟨by tauto, {refl := ?_, trans := ?_, antisymm := ?_}, ⟨?_⟩⟩;
-        . tauto;
-        . omega;
-        . simp only [M]; omega;
-        . simp only [Connected, and_imp, M]; omega;
-      . suffices ∃ x, (0 : M.World) ≺ x ∧ x ≠ 0 by
+      . exact {}
+      . suffices (0 : M) = 0 ∧ ∃ x, (0 : M.World) ≺ x ∧ x ≠ 0 by
           simpa [Semantics.Realize, Satisfies, ValidOnFrame, M];
-        use 1;
         constructor;
-        . omega;
-        . trivial;
+        . tauto;
+        . use 1;
+          constructor;
+          . omega;
+          . trivial;
 
 @[simp]
 theorem Triv.proper_extension_of_S4Point4M : Logic.S4Point4M ⊂ Logic.Triv := by
   constructor;
   . rw [S4Point4M.Kripke.preorder_sobocinski_mckinsey, Triv.Kripke.finite_equality];
-    rintro φ hφ F ⟨_, _⟩;
+    rintro φ hφ F hF;
     apply hφ;
-    refine ⟨by tauto, inferInstance, inferInstance⟩;
+    simp_all only [Set.mem_setOf_eq];
+    infer_instance;
   . suffices ∃ φ, Hilbert.Triv ⊢! φ ∧ ¬FrameClass.S4Point4M ⊧ φ by
       rw [S4Point4M.Kripke.preorder_sobocinski_mckinsey];
       tauto;
@@ -172,30 +157,33 @@ theorem Triv.proper_extension_of_S4Point4M : Logic.S4Point4M ⊂ Logic.Triv := b
       let M : Model := ⟨⟨Fin 2, λ x y => x ≤ y⟩, (λ w _ => w = 0)⟩;
       use M, 0;
       constructor;
-      . refine ⟨?_, ⟨?_⟩, ⟨?_⟩⟩;
-        . tauto;
-        . intro x y z _ Rxy Ryz;
-          match x, y, z with
-          | 0, 0, _ => contradiction;
-          | 1, 1, _ => contradiction;
-          | 0, 1, _ => omega
-          | 1, 0, _ => omega;
-        . intro x;
-          use 1;
-          simp [M];
-          constructor <;> omega;
-      . suffices ∃ x, (0 : M.World) ≺ x ∧ x ≠ 0 by
+      . exact {
+          refl := by tauto
+          sobocinski := by
+            intro x y z _ Rxy Ryz;
+            match x, y, z with
+            | 0, 0, _ => contradiction;
+            | 1, 1, _ => contradiction;
+            | 0, 1, _ => omega
+            | 1, 0, _ => omega;
+          mckinsey := by
+            intro x;
+            use 1;
+            simp [M];
+            constructor <;> omega;
+        }
+      . suffices (0 : M) = 0 ∧ ∃ x : M, (0 : M) ≺ x ∧ ¬x = 0 by
           simpa [Semantics.Realize, Satisfies, ValidOnFrame, M];
-        use 1;
         constructor;
-        . omega;
-        . trivial;
+        . tauto;
+        . use 1;
+          constructor;
+          . omega;
+          . trivial;
 
 @[simp]
-theorem Univ.proper_extension_of_Triv : Logic.Triv ⊂ Logic.Univ := by  constructor <;> simp;
+theorem Univ.proper_extension_of_Triv : Logic.Triv ⊂ Logic.Univ := by constructor <;> simp;
 
 end Logic
-
-
 
 end LO.Modal
