Foundation/Vorspiel/HRel/Equality.lean
@@ -3,51 +3,23 @@ import Foundation.Vorspiel.HRel.Connected
 
 variable {α} {R : HRel α}
 
-/-- States that `R` is `=` -/
-def Equality (R : HRel α) := ∀ ⦃x y⦄, R x y ↔ x = y
+class IsEquality (R : HRel α) extends IsRefl α R, IsCoreflexive R
 
-class IsEquality (R : HRel α) where
-  equality : Equality R
-
-instance [IsRefl _ R] [IsCoreflexive R] : IsEquality R := ⟨by
+@[simp]
+lemma equality [IsEquality R] : ∀ ⦃x y⦄, R x y ↔ x = y := by
   intro x y;
   constructor;
   . apply IsCoreflexive.corefl;
   . rintro rfl; apply IsRefl.refl;
-⟩
 
-instance [IsEquality R] : IsRefl α R := ⟨fun x ↦ IsEquality.equality.mpr (Eq.refl x)⟩
+instance [IsEquality R] : IsSymm α R := ⟨by simp_all⟩
 
-instance [IsEquality R] : IsCoreflexive R := ⟨fun _ _ Rxy ↦ IsEquality.equality.1 Rxy⟩
+instance [IsEquality R] : IsAntisymm α R := ⟨by simp_all⟩
 
-instance [IsEquality R] : IsSymm α R := ⟨by
-  intro x y Rxy;
-  replace Rxy := IsEquality.equality.1 Rxy; subst Rxy;
-  apply IsRefl.refl;
-⟩
+instance [IsEquality R] : IsTrans α R := ⟨by simp_all⟩
 
-instance [IsEquality R] : IsAntisymm α R := ⟨by
-  intro x y Rxy Ryx;
-  replace Rxy := IsEquality.equality.1 Rxy;
-  replace Ryx := IsEquality.equality.1 Ryx;
-  tauto;
-⟩
+instance [IsEquality R] : IsPiecewiseStronglyConnected R := ⟨by simp_all [PiecewiseStronglyConnected]⟩
 
-instance [IsEquality R] : IsTrans α R := ⟨by
-  rintro x y z Rxy Ryz;
-  replace Rxy := IsEquality.equality.1 Rxy;
-  replace Ryz := IsEquality.equality.1 Ryz;
-  subst Rxy Ryz;
-  apply refl;
-⟩
-
-instance [IsEquality R] : IsPiecewiseStronglyConnected R := ⟨by
-  rintro x y z Rxy Rxz;
-  replace Rxy := IsEquality.equality.1 Rxy;
-  replace Rxz := IsEquality.equality.1 Rxz;
-  subst Rxy Rxz;
-  left;
-  apply refl;
-⟩
-
-instance : IsEquality (α := α) (· = ·) := ⟨by intro x y; simp [Equality]⟩
+instance : IsEquality (α := α) (· = ·) where
+  refl := by simp
+  corefl := by simp [Coreflexive]
