Foundation/Modal/Boxdot/Grz_S.lean
@@ -1,14 +1,10 @@
 import Foundation.Modal.Boxdot.GL_Grz
 import Foundation.Modal.Boxdot.GL_S
 
-namespace LO
-
-namespace Modal.Logic
+namespace LO.Modal.Logic
 
 lemma iff_provable_Grz_provable_boxdot_S {φ : Formula _} : φ ∈ Logic.Grz ↔ φᵇ ∈ Logic.S := by
   apply Iff.trans iff_provable_boxdot_GL_provable_Grz.symm;
   exact iff_provable_boxdot_GL_provable_boxdot_S;
 
-end Modal.Logic
-
-end LO
+end LO.Modal.Logic
