Foundation/Modal/Boxdot/Ver_Triv.lean
@@ -4,7 +4,7 @@ import Foundation.Modal.Kripke.Logic.Ver
 
 namespace LO.Modal
 
-namespace Hilbert
+namespace Logic
 
 open Kripke
 open Formula.Kripke
@@ -12,28 +12,33 @@ open Formula (boxdotTranslate)
 open Modal.Kripke
 open LO.Entailment LO.Entailment.FiniteContext LO.Modal.Entailment
 
-lemma provable_boxdotTranslated_Ver_of_Triv : (Hilbert.Triv) ⊢! φ → (Hilbert.Ver) ⊢! φᵇ := boxdotTranslated_of_dominate $ by
-  intro φ hp;
+variable {φ : Formula ℕ}
+
+lemma provable_boxdotTranslated_Ver_of_Triv : φ ∈ Logic.Triv → φᵇ ∈ Logic.Ver := Hilbert.boxdotTranslated_of_dominate $ by
+  rintro φ hp;
   rcases (by simpa using hp) with (⟨_, _, rfl⟩ | ⟨_, rfl⟩ | ⟨_, rfl⟩);
   . exact boxdot_axiomK!;
   . simp only [boxdotTranslate, axiomVer!, and₁!];
   . apply deduct'!;
     apply K!_intro <;> simp;
 
-lemma provable_Triv_of_boxdotTranslated_Ver : (Hilbert.Ver) ⊢! φᵇ → (Hilbert.Triv) ⊢! φ := by
+lemma provable_Triv_of_boxdotTranslated_Ver : φᵇ ∈ Logic.Ver → φ ∈ Logic.Triv := by
   contrapose;
+  rw [Logic.Triv.Kripke.equality, Logic.Ver.Kripke.isolated];
   intro h;
-  obtain ⟨F, F_eq, h⟩ := iff_not_validOnFrameClass_exists_frame.mp $ (not_imp_not.mpr $ Hilbert.Triv.Kripke.complete_equality |>.complete) h;
+  obtain ⟨F, F_eq, h⟩ := iff_not_validOnFrameClass_exists_frame.mp $ h;
   replace F_eq := Set.mem_setOf_eq.mp F_eq;
-  apply not_imp_not.mpr $ Hilbert.Ver.Kripke.sound.sound;
   apply iff_not_validOnFrameClass_exists_frame.mpr;
   use F^≠;
   constructor;
-  . apply isIsolated_iff _ _ |>.mpr
-    intro x y;
-    by_contra hC;
-    obtain ⟨nxy, Rxy⟩ := hC;
-    exact nxy $ F_eq.equality.mp Rxy;
+  . exact {
+      isolated := by
+        intro x y;
+        by_contra hC;
+        obtain ⟨nxy, Rxy⟩ := hC;
+        apply nxy;
+        simpa using Rxy;
+    }
   . apply Kripke.iff_frame_boxdot_reflexive_closure.not.mpr;
     apply iff_reflexivize_irreflexivize'.not.mp;
     exact h;
@@ -43,8 +48,8 @@ theorem iff_boxdotTranslated_Ver_Triv : (Hilbert.Ver) ⊢! φᵇ ↔ (Hilbert.Tr
   provable_boxdotTranslated_Ver_of_Triv
 ⟩
 
-end Hilbert
+end Logic
 
-instance : BoxdotProperty (Logic.Ver) (Logic.Triv) := ⟨Hilbert.iff_boxdotTranslated_Ver_Triv⟩
+-- instance : BoxdotProperty (Logic.Ver) (Logic.Triv) := ⟨Hilbert.iff_boxdotTranslated_Ver_Triv⟩
 
 end LO.Modal
