Foundation/Modal/Kripke/Logic/S5.lean
@@ -31,7 +31,7 @@ instance [F.IsS5] : F.IsKTB where
 instance [F.IsS5] : F.IsS4Point4 where
 
 protected abbrev FrameClass.S5 : FrameClass := { F | F.IsS5 }
-protected abbrev FrameClass.finiteS5: FrameClass := { F | F.IsFiniteS5 }
+protected abbrev FrameClass.finite_S5: FrameClass := { F | F.IsFiniteS5 }
 protected abbrev FrameClass.universal : FrameClass := { F | F.IsUniversal }
 
 instance Frame.pointGenerate.isUniversal (F : Frame) (r : F.World) (_ : F.IsS5) : (F↾r).IsUniversal where
